Sequences/NatSeqConversions.dfy
@@ -2,37 +2,28 @@ include "NatSeq.dfy"
 
 abstract module NatSeqConversions refines NatSeq {
 
-  function method BASE1(): nat
-		ensures BASE1() > 1
-  type uint1 = i: int | 0 <= i < BASE1()
+  import NatSeq1
+  import NatSeq2
 
-  function method BASE2(): nat
-		ensures BASE2() > 1
-  type uint2 = i: int | 0 <= i < BASE2()
-
-  function method BASE(): nat { BASE2() }
-
-  function {:opaque} to_smaller_base(xs: seq<uint1>): seq<uint2>
-    requires exists n :: BASE1() == power(BASE2(), n) && n > 1
+  function {:opaque} to_lower_base(xs: seq<NatSeq1.uint>): seq<NatSeq2.uint>
   {
     if xs == [] then []
-    else to_seq(first(xs)) + to_smaller_base(drop_first(xs))
+    else NatSeq2.to_seq(first(xs)) + to_lower_base(drop_first(xs))
   }
 
-  function {:opaque} to_larger_base(xs: seq<uint2>): seq<uint1>
-    requires exists n :: BASE1() == power(BASE2(), n) && n > 1
+  function {:opaque} to_higher_base(xs: seq<NatSeq2.uint>): seq<NatSeq1.uint>
   {
     if xs == [] then []
     else
-      var n: nat :| BASE1() == power(BASE2(), n) && n > 1;
+      var n: nat :| NatSeq1.BASE() == power(NatSeq2.BASE(), n) && n > 1;
       if |xs| < n then
-        lemma_seq_nat_bound(xs);
-        lemma_power_strictly_increases(BASE2(), |xs|, n);
-        [to_nat(xs) as uint1]
+        NatSeq2.lemma_seq_nat_bound(xs);
+        lemma_power_strictly_increases(NatSeq2.BASE(), |xs|, n);
+        [NatSeq2.to_nat(xs) as NatSeq1.uint]
       else
-        lemma_seq_nat_bound(xs[..n]);
+        NatSeq2.lemma_seq_nat_bound(xs[..n]);
         lemma_mod_sub_multiples_vanish_auto();
-        [to_nat(xs[..n]) as uint1] + to_larger_base(xs[n..])
+        [NatSeq2.to_nat(xs[..n]) as NatSeq1.uint] + to_higher_base(xs[n..])
   }
 
 }
